Keep only the definition of parallel interference

model/basic/interference.v
@@ -73,7 +73,8 @@ Module Interference.
       (* Let job_other be a job that interferes with j. *)
       Variable job_other: JobIn arr_seq.
 
-      (* The interference caused by job_other is defined as follows. *)
+      (* We define the total interference caused by job_other during [t1, t2) as the
+         cumulative service received by job_other while j is backlogged. *)
       Definition job_interference (t1 t2: time) :=
         \sum_(t1 <= t < t2)
           \sum_(cpu < num_cpus)
@@ -81,65 +82,28 @@ Module Interference.
 
     End JobInterference.
 
-    Section JobInterferenceSequential.
-
-      (* Let job_other be a job that interferes with j. *)
-      Variable job_other: JobIn arr_seq.
-
-      (* If jobs are sequential, the interference caused by job_other
-         is defined as follows. *)
-      Definition job_interference_sequential (t1 t2: time) :=
-        \sum_(t1 <= t < t2)
-         (job_is_backlogged t && scheduled sched job_other t).
-
-    End JobInterferenceSequential.
-
     Section TaskInterference.
 
       (* In order to define task interference, consider any interfering task tsk_other. *)
       Variable tsk_other: sporadic_task.
       
-      Definition schedules_job_of_task (cpu: processor num_cpus) (t: time) :=
-        match (sched cpu t) with
-          | Some j' => job_task j' == tsk_other
-          | None => false
-        end.
-
-      (* We know that tsk is scheduled at time t if there exists a processor
-         scheduling a job of tsk. *)
-      Definition task_is_scheduled (t: time) :=
-        [exists cpu in processor num_cpus, schedules_job_of_task cpu t].
-
-      (* We define the total interference caused by tsk during [t1, t2) as the
-         cumulative time in which j is backlogged while tsk is scheduled. *)
+      (* We define the total interference caused by tsk during [t1, t2) as
+         the cumulative service received by tsk while j is backlogged. *)
       Definition task_interference (t1 t2: time) :=
         \sum_(t1 <= t < t2)
           \sum_(cpu < num_cpus)
-            (job_is_backlogged t && schedules_job_of_task cpu t).
+            (job_is_backlogged t &&
+            task_scheduled_on job_task sched tsk_other cpu t).
 
     End TaskInterference.
-
-    Section TaskInterferenceSequential.
-
-      (* In order to define task interference, consider any interfering task tsk_other. *)
-      Variable tsk_other: sporadic_task.
-    
-      (* If jobs are sequential, we define the total interference caused by
-         tsk during [t1, t2) as the cumulative time in which j is backlogged
-         while tsk is scheduled. *)
-      Definition task_interference_sequential (t1 t2: time) :=
-        \sum_(t1 <= t < t2)
-          (job_is_backlogged t && task_is_scheduled tsk_other t).
-
-    End TaskInterferenceSequential.
 
     Section TaskInterferenceJobList.
 
       Variable tsk_other: sporadic_task.
 
-      Definition task_interference_sequential_joblist (t1 t2: time) :=
+      Definition task_interference_joblist (t1 t2: time) :=
         \sum_(j <- jobs_scheduled_between sched t1 t2 | job_task j == tsk_other)
-         job_interference_sequential j t1 t2.
+         job_interference j t1 t2.
 
     End TaskInterferenceJobList.
 
@@ -156,29 +120,6 @@ Module Interference.
         by rewrite big_const_nat iter_addn mul1n addn0 leqnn.
       Qed.
 
-      Lemma job_interference_seq_le_delta :
-        forall j_other t1 delta,
-          job_interference_sequential j_other t1 (t1 + delta) <= delta.
-      Proof.
-        unfold job_interference; intros j_other t1 delta.
-        apply leq_trans with (n := \sum_(t1 <= t < t1 + delta) 1);
-          first by apply leq_sum; ins; apply leq_b1.
-        by rewrite big_const_nat iter_addn mul1n addn0 addKn leqnn.
-      Qed.
-
-      Lemma job_interference_seq_le_service :
-        forall j_other t1 t2,
-          job_interference_sequential j_other t1 t2 <= service_during sched j_other t1 t2.
-      Proof.
-        intros j_other t1 t2; unfold job_interference_sequential, service_during.
-        apply leq_trans with (n := \sum_(t1 <= t < t2) scheduled sched j_other t);
-          first by apply leq_sum; ins; destruct (job_is_backlogged i); rewrite ?andTb ?andFb.
-        apply leq_sum; intros t _.
-        destruct (scheduled sched j_other t) eqn:SCHED; last by done.
-        move: SCHED => /existsP EX; destruct EX as [cpu]; move: H => /andP [IN SCHED].
-        unfold service_at; rewrite (bigD1 cpu); last by done.
-        by apply leq_trans with (n := 1).
-      Qed.
 
       Lemma job_interference_le_service :
         forall j_other t1 t2,
@@ -192,23 +133,6 @@ Module Interference.
         by destruct (scheduled_on sched j_other cpu t).
       Qed.
       
-      Lemma task_interference_seq_le_workload :
-        forall tsk t1 t2,
-          task_interference_sequential tsk t1 t2 <= workload job_task sched tsk t1 t2.
-      Proof.
-        unfold task_interference, workload; intros tsk t1 t2.
-        apply leq_sum; intros t _.
-        rewrite -mulnb -[\sum_(_ < _) _]mul1n.
-        apply leq_mul; first by apply leq_b1.
-        destruct (task_is_scheduled tsk t) eqn:SCHED; last by ins.
-        unfold task_is_scheduled in SCHED.
-        move: SCHED =>/exists_inP SCHED.
-        destruct SCHED as [cpu _ HAScpu].
-        rewrite -> bigD1 with (j := cpu); simpl; last by ins.
-        apply ltn_addr; unfold service_of_task, schedules_job_of_task in *.
-        by destruct (sched cpu t); [rewrite HAScpu | by done].
-      Qed.
-
       Lemma task_interference_le_workload :
         forall tsk t1 t2,
           task_interference tsk t1 t2 <= workload job_task sched tsk t1 t2.
@@ -217,135 +141,85 @@ Module Interference.
         apply leq_sum; intros t _.
         apply leq_sum; intros cpu _.
         destruct (job_is_backlogged t); [rewrite andTb | by rewrite andFb].
-        unfold schedules_job_of_task, service_of_task.
+        unfold task_scheduled_on, service_of_task.
         by destruct (sched cpu t).
       Qed.
 
     End BasicLemmas.
 
-    (* The sequential per-job interference bounds the actual interference. *)
-    Section BoundUsingPerJobInterference.
+    Section InterferenceSequentialJobs.
 
-      Lemma interference_le_interference_joblist :
-        forall tsk t1 t2,
-          task_interference_sequential tsk t1 t2 <=
-          task_interference_sequential_joblist tsk t1 t2.
+      (* If jobs are sequential, ... *)
+      Hypothesis H_sequential_jobs: sequential_jobs sched.
+    
+      (* ... then the interference incurred by a job in an interval
+         of length delta is at most delta. *)
+      Lemma job_interference_le_delta :
+        forall j_other t1 delta,
+          job_interference j_other t1 (t1 + delta) <= delta.
       Proof.
-        intros tsk t1 t2; unfold task_interference_sequential, task_interference_sequential_joblist, job_interference.
-        rewrite [\sum_(j <- jobs_scheduled_between _ _ _ | _) _]exchange_big /=.
-        rewrite big_nat_cond [\sum_(_ <= _ < _ | true)_]big_nat_cond.
-        apply leq_sum; intro t; rewrite andbT; intro LT.
-        destruct (job_is_backlogged t && task_is_scheduled tsk t) eqn:BACK;
-          last by done.
-        move: BACK => /andP [BACK SCHED].
-        move: SCHED => /existsP SCHED; destruct SCHED as [x IN]; move: IN => /andP [IN SCHED].
-        unfold schedules_job_of_task in SCHED; desf.
-        rename SCHED into EQtsk0, Heq into SCHED; move: EQtsk0 => /eqP EQtsk0.
-        rewrite big_mkcond (bigD1_seq j0) /=; last by rewrite undup_uniq.
+        rename H_sequential_jobs into SEQ.
+        unfold job_interference, sequential_jobs in *.
+        intros j_other t1 delta.
+        apply leq_trans with (n := \sum_(t1 <= t < t1 + delta) 1);
+          last by rewrite big_const_nat iter_addn mul1n addn0 addKn leqnn.
+        apply leq_sum; intros t _.
+        destruct ([exists cpu, scheduled_on sched j_other cpu t]) eqn:EX.
         {
-          rewrite -addn1 addnC; apply leq_add; last by done.
-          rewrite EQtsk0 BACK andTb.
-          apply eq_leq; symmetry; apply/eqP; rewrite eqb1.
-          unfold scheduled, scheduled_on.
-          by apply/exists_inP; exists x; [by done | by rewrite SCHED].
+          move: EX => /existsP [cpu SCHED].
+          rewrite (bigD1 cpu) // /=.
+          rewrite big_mkcond (eq_bigr (fun x => 0)) /=;
+            first by simpl_sum_const; rewrite leq_b1.
+          intros cpu' _; des_if_goal; last by done.
+          destruct (scheduled_on sched j_other cpu' t) eqn:SCHED'; last by rewrite andbF.
+          move: SCHED SCHED' => /eqP SCHED /eqP SCHED'.
+          by specialize (SEQ j_other t cpu cpu' SCHED SCHED'); rewrite SEQ in Heq.
+        }
+        {
+          apply negbT in EX; rewrite negb_exists in EX.
+          move: EX => /forallP EX.
+          rewrite (eq_bigr (fun x => 0)); first by simpl_sum_const.
+          by intros cpu _; specialize (EX cpu); apply negbTE in EX; rewrite EX andbF.
+        }
+      Qed.
+
+    End InterferenceSequentialJobs.
+
+    (* The sequential per-job interference bounds the actual interference. *)    
+    Section BoundUsingPerJobInterference.
+    Lemma interference_le_interference_joblist :
+        forall tsk t1 t2,
+          task_interference tsk t1 t2 <= task_interference_joblist tsk t1 t2.
+      Proof.
+        intros tsk t1 t2.
+        unfold task_interference, task_interference_joblist, job_interference, job_is_backlogged.
+        rewrite [\sum_(_ <- _ sched _ _ | _) _]exchange_big /=.
+        rewrite big_nat_cond [\sum_(_ <= _ < _ | true) _]big_nat_cond.
+        apply leq_sum; move => t /andP [LEt _].
+        rewrite exchange_big /=.
+        apply leq_sum; intros cpu _.
+        destruct (backlogged job_cost sched j t) eqn:BACK;      
+          last by rewrite andFb (eq_bigr (fun x => 0));
+            first by rewrite big_const_seq iter_addn mul0n addn0.
+        rewrite andTb.
+        destruct (task_scheduled_on job_task sched tsk cpu t) eqn:SCHED; last by done.
+        unfold scheduled_on, task_scheduled_on in *.
+        destruct (sched cpu t) as [j' |] eqn:SOME; last by done.
+        rewrite big_mkcond /= (bigD1_seq j') /=; last by apply undup_uniq.
+        {
+          by rewrite SCHED eq_refl.
         }
         {
           unfold jobs_scheduled_between.
-          rewrite mem_undup.
-          apply mem_bigcat_nat with (j := t); first by auto.
-          unfold jobs_scheduled_at.
-          apply mem_bigcat_ord with (j := x); first by apply ltn_ord.
-          by unfold make_sequence; rewrite SCHED mem_seq1 eq_refl.
+          rewrite mem_undup; apply mem_bigcat_nat with (j := t);
+            first by done.
+          apply mem_bigcat_ord with (j := cpu); first by apply ltn_ord.
+          by unfold make_sequence; rewrite SOME mem_seq1 eq_refl.
         }
       Qed.
         
     End BoundUsingPerJobInterference.
-
-    Section CorrespondenceWithService.
-
-      Variable t1 t2: time.
-      
-      (* Assume that jobs are sequential, ...*)
-      Hypothesis H_sequential_jobs: sequential_jobs sched.
-
-      (* ..., and that jobs only execute after they arrived
-         and no longer than their execution costs. *)
-      Hypothesis H_jobs_must_arrive_to_execute:
-        jobs_must_arrive_to_execute sched.
-      Hypothesis H_completed_jobs_dont_execute:
-        completed_jobs_dont_execute job_cost sched.
-
-      (* If job j had already arrived at time t1 and did not yet
-         complete by time t2, ...*)
-      Hypothesis H_job_has_arrived :
-        has_arrived j t1.
-      Hypothesis H_job_is_not_complete :
-        ~~ completed job_cost sched j t2.
-
-      (* ... then the service received by j during [t1, t2) equals
-         the cumulative time in which it did not incur interference. *)
-      Lemma complement_of_interf_equals_service :
-        \sum_(t1 <= t < t2) service_at sched j t =
-          t2 - t1 - total_interference t1 t2.
-      Proof.
-        unfold completed, total_interference, job_is_backlogged,
-               backlogged, service_during, pending.
-        rename H_sequential_jobs into NOPAR,
-               H_jobs_must_arrive_to_execute into MUSTARRIVE,
-               H_completed_jobs_dont_execute into COMP,
-               H_job_is_not_complete into NOTCOMP.
-
-        (* Reorder terms... *)
-        apply/eqP; rewrite subh4; first last.
-        {
-          rewrite -[t2 - t1]mul1n -[1*_]addn0 -iter_addn -big_const_nat.
-          by apply leq_sum; ins; apply leq_b1.
-        }
-        {
-          rewrite -[t2 - t1]mul1n -[1*_]addn0 -iter_addn -big_const_nat.
-          by apply leq_sum; ins; apply service_at_most_one. 
-        }
-        apply/eqP.
-        
-        apply eq_trans with (y := \sum_(t1 <= t < t2)
-                                    (1 - service_at sched j t));
-          last first.
-        {
-          apply/eqP; rewrite <- eqn_add2r with (p := \sum_(t1 <= t < t2)
-                                               service_at sched j t).
-          rewrite subh1; last first.
-            rewrite -[t2 - t1]mul1n -[1*_]addn0 -iter_addn -big_const_nat.
-            by apply leq_sum; ins; apply service_at_most_one.
-          rewrite -addnBA // subnn addn0 -big_split /=.
-          rewrite -[t2 - t1]mul1n -[1*_]addn0 -iter_addn -big_const_nat.
-          apply/eqP; apply eq_bigr; ins; rewrite subh1;
-            [by rewrite -addnBA // subnn addn0 | by apply service_at_most_one].
-        }
-        rewrite big_nat_cond [\sum_(_ <= _ < _ | true)_]big_nat_cond.
-        apply eq_bigr; intro t; rewrite andbT; move => /andP [GEt1 LTt2].
-        destruct (~~ scheduled sched j t) eqn:SCHED; last first.
-        {
-          apply negbFE in SCHED; unfold scheduled in *.
-          move: SCHED => /exists_inP SCHED; destruct SCHED as [cpu INcpu SCHEDcpu].
-          rewrite andbF; apply/eqP.
-          rewrite -(eqn_add2r (service_at sched j t)) add0n.
-          rewrite subh1; last by apply service_at_most_one.
-          rewrite -addnBA // subnn addn0.
-          rewrite eqn_leq; apply/andP; split; first by apply service_at_most_one.
-          unfold service_at; rewrite (bigD1 cpu) /=; last by apply SCHEDcpu.
-          by apply leq_trans with (n := 1).
-        }
-        rewrite not_scheduled_no_service in SCHED.
-        move: SCHED => /eqP SCHED.
-        rewrite SCHED subn0 andbT; apply/eqP; rewrite eqb1.
-        apply/andP; split; first by apply leq_trans with (n := t1).
-        apply/negP; unfold not; intro BUG.
-        apply completion_monotonic with (t' := t2) in BUG; [ | by ins | by apply ltnW].
-        by rewrite BUG in NOTCOMP.
-      Qed.
-      
-    End CorrespondenceWithService.
-
+    
   End InterferenceDefs.
 
 End Interference.
