analysis/jitter/bertogna_edf_theory.v
@@ -10,7 +10,7 @@ Require Import ssreflect ssrbool eqtype ssrnat seq fintype bigop div path.
 
 Module ResponseTimeAnalysisEDFJitter.
 
-  Export JobWithJitter SporadicTaskset ScheduleWithJitter ScheduleOfSporadicTask Workload
+  Export JobWithJitter SporadicTaskset ScheduleOfSporadicTaskWithJitter Workload
          Schedulability ResponseTime Priority SporadicTaskArrival WorkloadBoundJitter
          InterferenceBoundEDFJitter Platform Interference.
 
@@ -228,50 +228,44 @@ Module ResponseTimeAnalysisEDFJitter.
         Lemma bertogna_edf_too_much_interference : X >= R - task_cost tsk + 1.
         Proof.
           rename H_completed_jobs_dont_execute into COMP,
-                 H_valid_job_parameters into PARAMS,
-                 H_job_of_tsk into JOBtsk,
-                 H_j_not_completed into NOTCOMP.
+                 H_valid_job_parameters into PARAMS, H_response_time_is_fixed_point into REC,
+                 H_job_of_tsk into JOBtsk, H_j_not_completed into NOTCOMP.
           unfold completed, valid_sporadic_job_with_jitter, valid_sporadic_job in *.
-
-          (* Since j has not completed, recall the time when it is not
-           executing is the total interference. *)
-          exploit (complement_of_interf_equals_service job_cost job_jitter sched j t1 (t1 + R));
-            try (by done); first by apply leqnn. 
-          intros EQinterf.
-          rewrite {2}[_ + R]addnC -addnBA // subnn addn0 in EQinterf.
-          rewrite addn1.
-          move: NOTCOMP; rewrite neq_ltn; move => /orP NOTCOMP; des;
-            last first.
+          unfold X, total_interference; rewrite addn1.
+          rewrite -(ltn_add2r (task_cost tsk)).
+          rewrite subh1; last by rewrite [R](REC tsk) // leq_addr.
+          rewrite -addnBA // subnn addn0.
+          move: (NOTCOMP) => /negP NOTCOMP'.
+          rewrite neq_ltn in NOTCOMP.
+          move: NOTCOMP => /orP [LT | BUG]; last first.
           {
-            apply (leq_ltn_trans (COMP j (t1 + R))) in NOTCOMP.
-            by rewrite ltnn in NOTCOMP.
+            exfalso; rewrite ltnNge in BUG; move: BUG => /negP BUG; apply BUG.
+            by apply cumulative_service_le_job_cost.
           }
-          apply leq_trans with (n := R - service sched j (t1 + R)); last first.
+          apply leq_ltn_trans with (n := (\sum_(t1 <= t < t1 + R)
+                                       backlogged job_cost job_jitter sched j t) +
+                                     service sched j (t1 + R)); last first.
           {
-            unfold service.
-            rewrite -> big_cat_nat with (n := t1); [simpl | by done | by apply leq_addr].
-            rewrite -> cumulative_service_before_jitter_zero with (job_jitter0 := job_jitter);
-              [rewrite add0n | by done | by apply leqnn].
-            rewrite EQinterf subKn; first by done.
-            {
-              unfold total_interference.
-              apply leq_trans with (n := \sum_(t1 <= t < t1 + R) 1);
-                first by apply leq_sum; ins; apply leq_b1.
-              rewrite big_const_nat iter_addn mul1n addn0.
-              by rewrite addnC -addnBA // subnn addn0.
-            }
+            rewrite -addn1 -addnA leq_add2l addn1.
+            apply leq_trans with (n := job_cost j); first by done.
+            by specialize (PARAMS j); des; rewrite -JOBtsk.
           }
-          {
-            apply ltn_sub2l; last first.
-            {
-              apply leq_trans with (n := job_cost j); first by ins.
-              rewrite -JOBtsk; specialize (PARAMS j); des; apply PARAMS1.
-            }
-            apply leq_trans with (n := job_cost j); first by ins.
-            apply leq_trans with (n := task_cost tsk);
-              first by rewrite -JOBtsk; specialize (PARAMS j); des; apply PARAMS1.
-            by rewrite bertogna_edf_R_other_ge_cost.
-          }
+          unfold service.
+          rewrite -> big_cat_nat with (n := t1) (m := 0); rewrite ?leq_addr // /=.
+          rewrite (cumulative_service_before_jitter_zero job_jitter) // add0n.
+          rewrite -big_split /=.
+          apply leq_trans with (n := \sum_(t1 <= i < t1 + R) 1);
+            first by simpl_sum_const; rewrite addKn.
+          apply leq_sum_nat; move => i /andP [GEi LTi] _.
+          destruct (backlogged job_cost job_jitter sched j i) eqn:BACK;
+            first by rewrite -addn1 addnC; apply leq_add.
+          apply negbT in BACK.
+          rewrite add0n lt0n -not_scheduled_no_service negbK.
+          rewrite /backlogged negb_and negbK in BACK.
+          move: BACK => /orP [/negP NOTPENDING | SCHED]; last by done.
+          exfalso; apply NOTPENDING; unfold pending; apply/andP; split; first by done.
+          apply/negP; red; intro BUG; apply NOTCOMP'.
+          by apply completion_monotonic with (t := i); try (by done); apply ltnW.
         Qed.
 
         Let scheduled_task_other_than_tsk (t: time) (tsk_other: sporadic_task) :=
@@ -296,13 +290,12 @@ Module ResponseTimeAnalysisEDFJitter.
                  H_rt_bounds_contains_all_tasks into UNZIP,
                  H_constrained_deadlines into RESTR,
                  H_work_conserving into WORK.
-          unfold valid_sporadic_job_with_jitter, valid_sporadic_job in *.
+          unfold x, X, total_interference, task_interference,
+                 valid_sporadic_job_with_jitter, valid_sporadic_job in *.
           move => t /andP [LEt LTt] BACK.
           unfold scheduled_task_other_than_tsk in *.
           eapply platform_cpus_busy_with_interfering_tasks; try (by done);
-            [ by apply WORK
-            | by done
-            | by apply SPO 
+            [ by apply WORK | by done | by apply SPO 
             | apply PARAMS; rewrite -JOBtsk; apply FROMTS
             | by apply JOBtsk | by apply BACK | ].
           {
@@ -332,7 +325,80 @@ Module ResponseTimeAnalysisEDFJitter.
           }
         Qed.
       
-        (* 2) Next, we prove that the sum of the interference of each task is equal
+        (* 2) Prove that during the scheduling window of j, any job that is scheduled while j is
+           backlogged comes from a different task. *)
+        Lemma bertogna_edf_interference_by_different_tasks :
+          forall t j_other,
+            t1 <= t < t1 + R ->
+            backlogged job_cost job_jitter sched j t ->
+            scheduled sched j_other t ->
+            job_task j_other != tsk.
+        Proof.
+          rename H_all_jobs_from_taskset into FROMTS,
+                 H_valid_task_parameters into PARAMS,
+                 H_valid_job_parameters into JOBPARAMS,
+                 H_job_of_tsk into JOBtsk, H_sporadic_tasks into SPO,
+                 H_work_conserving into WORK,
+                 H_tsk_R_in_rt_bounds into INbounds,
+                 H_all_previous_jobs_completed_on_time into BEFOREok,
+                 H_tasks_miss_no_deadlines into NOMISS,
+                 H_constrained_deadlines into CONSTR.
+          unfold valid_sporadic_job_with_jitter, valid_sporadic_job in *.
+          move => t j_other /andP [LEt GEt] BACK SCHED.
+          apply/eqP; red; intro SAMEtsk.
+          move: SCHED => /existsP [cpu SCHED].
+          assert (SCHED': scheduled sched j_other t).
+            by apply/existsP; exists cpu.
+          clear SCHED; rename SCHED' into SCHED.
+          move: (SCHED) => PENDING.
+          apply scheduled_implies_pending with (job_cost0 := job_cost) (job_jitter0 := job_jitter)
+            in PENDING; try (by done).
+          destruct (ltnP (job_arrival j_other) (job_arrival j)) as [BEFOREother | BEFOREj].
+          {
+            move: (BEFOREother) => LT; rewrite -(ltn_add2r R) in LT.
+            exploit (BEFOREok j_other tsk R SAMEtsk INbounds).
+            {
+              rewrite -addnA [_ + R]addnC addnA -[(_ + _) + R]addnA [_ tsk + R]addnC addnA.
+              by rewrite ltn_add2r.
+            }
+            intros COMP.
+            move: PENDING => /andP [_ /negP NOTCOMP]; apply NOTCOMP.
+            apply completion_monotonic with (t0 := job_arrival j_other + task_jitter tsk + R);
+              try by done.
+            apply leq_trans with (n := job_arrival j);
+              last by apply leq_trans with (n := t1); [by apply leq_addr | by done].
+            apply leq_trans with (n := job_arrival j_other + task_period tsk).
+            {
+              rewrite -addnA leq_add2l.
+              by apply leq_trans with (n := task_deadline tsk);
+                [by apply NOMISS | by apply CONSTR; rewrite -JOBtsk FROMTS].
+            }
+            rewrite -SAMEtsk; apply SPO; [ | by rewrite JOBtsk | by apply ltnW].
+            by red; intro EQ; subst; rewrite ltnn in BEFOREother.
+          }
+          {
+            move: PENDING => /andP [ARRIVED _].
+            exploit (SPO j j_other); [ | by rewrite SAMEtsk | by done | ]; last first.
+            {
+              apply/negP; rewrite -ltnNge JOBtsk.
+              apply leq_trans with (n := job_arrival j + task_deadline tsk);
+                last by rewrite leq_add2l; apply CONSTR; rewrite -JOBtsk FROMTS.
+              apply leq_trans with (n := job_arrival j + task_jitter tsk + R);
+                last by rewrite -addnA leq_add2l; apply NOMISS.
+              apply leq_trans with (n := t1 + R); last first.
+              {
+                rewrite leq_add2r leq_add2l -JOBtsk.
+                by specialize (JOBPARAMS j); des.
+              }
+              apply leq_ltn_trans with (n := job_arrival j_other + job_jitter j_other);
+                first by apply leq_addr.
+              by apply leq_ltn_trans with (n := t).
+            }
+            by intros EQtsk; subst j_other; rewrite /backlogged SCHED andbF in BACK.
+          }
+        Qed.
+
+      (* 3) Next, we prove that the sum of the interference of each task is equal
           to the total interference multiplied by the number of processors. This
           holds because interference only occurs when all processors are busy. *)
         Lemma bertogna_edf_all_cpus_busy :
@@ -340,43 +406,87 @@ Module ResponseTimeAnalysisEDFJitter.
         Proof.
           rename H_all_jobs_from_taskset into FROMTS,
                  H_valid_task_parameters into PARAMS,
-                 H_valid_job_parameters into JOBPARAMS,
-                 H_job_of_tsk into JOBtsk,
-                 H_sporadic_tasks into SPO,
+                 H_job_of_tsk into JOBtsk, H_sporadic_tasks into SPO,
+                 H_work_conserving into WORK,
                  H_tsk_R_in_rt_bounds into INbounds,
                  H_all_previous_jobs_completed_on_time into BEFOREok,
                  H_tasks_miss_no_deadlines into NOMISS,
-                 H_constrained_deadlines into RESTR.
-          unfold sporadic_task_model, valid_sporadic_job_with_jitter, valid_sporadic_job in *.
+                 H_rt_bounds_contains_all_tasks into UNZIP,
+                 H_constrained_deadlines into CONSTR.
+          unfold sporadic_task_model in *.
           unfold x, X, total_interference, task_interference.
-          rewrite -big_mkcond -exchange_big big_distrl /=.
+          rewrite -big_mkcond -exchange_big big_distrl /= mul1n.
           rewrite [\sum_(_ <= _ < _ | backlogged _ _ _ _ _) _]big_mkcond.
-          apply eq_big_nat; move => t LEt.
+          apply eq_big_nat; move => t /andP [GEt LTt].
           destruct (backlogged job_cost job_jitter sched j t) eqn:BACK;
-            last by rewrite (eq_bigr (fun i => 0));
-              [by rewrite big_const_seq iter_addn mul0n addn0 | by done].
-          rewrite big_mkcond mul1n /=.
-          rewrite big_filter big_mkcond.
-          rewrite (eq_bigr (fun i => if (scheduled_task_other_than_tsk t i) then 1 else 0)); last first.
+            last by rewrite big1 //; ins; rewrite big1.
+          rewrite big_mkcond /=.
+          rewrite exchange_big /=.
+          apply eq_trans with (y := \sum_(cpu < num_cpus) 1); last by simpl_sum_const.
+          apply eq_bigr; intros cpu _.
+          move: (WORK j t BACK cpu) => [j_other /eqP SCHED]; unfold scheduled_on in *.
+          rewrite (bigD1_seq (job_task j_other)) /=; last by rewrite filter_uniq.
           {
-            unfold scheduled_task_other_than_tsk; intros i _; clear -i.
-            by destruct (task_is_scheduled job_task sched i t);
-              rewrite ?andFb ?andTb ?andbT //; desf.
+            rewrite (eq_bigr (fun i => 0));
+              last by intros i DIFF; rewrite /task_scheduled_on SCHED;apply/eqP;rewrite eqb0 eq_sym.
+            simpl_sum_const; apply/eqP; rewrite eqb1.
+            by unfold task_scheduled_on; rewrite SCHED.
           }
-          rewrite -big_mkcond sum1_count.
-          by apply bertogna_edf_scheduling_invariant.
+          rewrite mem_filter; apply/andP; split; last by apply FROMTS.
+          unfold jldp_can_interfere_with.
+          apply bertogna_edf_interference_by_different_tasks with (t := t); [by auto | by done |].
+          by apply/existsP; exists cpu; apply/eqP.
         Qed.
 
+        (* 4) Show that by the induction hypothesis, all jobs released
+           before the end of the interval complete by their periods. *)
+        Lemma bertogna_edf_all_previous_jobs_complete_by_their_period:
+          forall t (j0: JobIn arr_seq),
+            t < t1 + R ->
+            job_arrival j0 + task_period (job_task j0) <= t ->
+            completed job_cost sched j0
+               (job_arrival j0 + task_period (job_task j0)).
+        Proof.
+          rename H_valid_job_parameters into JOBPARAMS,
+                 H_rt_bounds_contains_all_tasks into UNZIP,
+                 H_job_of_tsk into JOBtsk,
+                 H_constrained_deadlines into CONSTR,
+                 H_tasks_miss_no_deadlines into NOMISS,
+                 H_all_jobs_from_taskset into FROMTS,
+                 H_all_previous_jobs_completed_on_time into BEFOREok.
+          unfold valid_sporadic_job_with_jitter, valid_sporadic_job in *.
+          intros t j0 LEt LE.
+          cut ((job_task j0) \in unzip1 rt_bounds); [intro IN | by rewrite UNZIP FROMTS].
+          move: IN => /mapP [p IN EQ]; destruct p as [tsk' R0]; simpl in *; subst tsk'.
+          apply completion_monotonic with (t0 := job_arrival j0 +
+                                        task_jitter (job_task j0) + R0); first by done.
+          {
+            rewrite -addnA leq_add2l.
+            apply leq_trans with (n := task_deadline (job_task j0));
+              [by apply NOMISS | by apply CONSTR; rewrite FROMTS].
+          }
+          apply BEFOREok with (tsk_other := (job_task j0)); try by done.
+          apply leq_ltn_trans with (n := t); last first.
+          {
+            apply leq_trans with (n := t1 + R); first by done.
+            rewrite leq_add2r leq_add2l -JOBtsk.
+            by specialize (JOBPARAMS j); des.
+          }
+          apply leq_trans with (n := job_arrival j0 + task_period (job_task j0)); last by done.
+          by rewrite -addnA leq_add2l; apply leq_trans with (n := task_deadline (job_task j0));
+            [by apply NOMISS | apply CONSTR; rewrite FROMTS].
+        Qed.
+        
         (* Let (cardGE delta) be the number of interfering tasks whose interference
            is larger than delta. *)
         Let cardGE (delta: time) := count (fun i => x i >= delta) ts_interf.
 
-        (* 3) If there is at least one of such tasks (e.g., cardGE > 0), then the
+        (* 5) If there is at least one of such tasks (e.g., cardGE > 0), then the
            cumulative interference caused by the complementary set of interfering
            tasks fills at least (num_cpus - cardGE) processors. *)
         Lemma bertogna_edf_helper_lemma :
           forall delta,
-            cardGE delta > 0 ->
+            0 < cardGE delta < num_cpus ->
             \sum_(i <- ts_interf | x i < delta) x i >= delta * (num_cpus - cardGE delta).
         Proof.
           rename H_all_jobs_from_taskset into FROMTS,
@@ -386,19 +496,21 @@ Module ResponseTimeAnalysisEDFJitter.
                  H_tsk_R_in_rt_bounds into INbounds,
                  H_all_previous_jobs_completed_on_time into BEFOREok,
                  H_tasks_miss_no_deadlines into NOMISS,
-                 H_constrained_deadlines into RESTR.
+                 H_constrained_deadlines into CONSTR,
+                 H_sequential_jobs into SEQ.
           unfold sporadic_task_model in *.
-          intros delta HAS.
+          move => delta /andP [HAS LT]. 
+          rewrite -has_count in HAS.
+
           set some_interference_A := fun t =>
-              backlogged job_cost job_jitter sched j t &&
-              has (fun tsk_k => ((x tsk_k >= delta) &&
-                       task_is_scheduled job_task sched tsk_k t)) ts_interf.      
+            has (fun tsk_k => backlogged job_cost job_jitter sched j t &&
+                              (x tsk_k >= delta) &&
+                              task_is_scheduled job_task sched tsk_k t) ts_interf.
           set total_interference_B := fun t =>
               backlogged job_cost job_jitter sched j t *
               count (fun tsk_k => (x tsk_k < delta) &&
-                task_is_scheduled job_task sched tsk_k t) ts_interf.
+                    task_is_scheduled job_task sched tsk_k t) ts_interf.
 
-          rewrite -has_count in HAS.
           apply leq_trans with ((\sum_(t1 <= t < t1 + R)
                                 some_interference_A t) * (num_cpus - cardGE delta)).
           {
@@ -406,39 +518,69 @@ Module ResponseTimeAnalysisEDFJitter.
             move: HAS => /hasP HAS; destruct HAS as [tsk_a INa LEa].
             apply leq_trans with (n := x tsk_a); first by apply LEa.
             unfold x, task_interference, some_interference_A.
-            apply leq_sum; ins.
-            destruct (backlogged job_cost job_jitter sched j i);
-              [rewrite 2!andTb | by ins].
-            destruct (task_is_scheduled job_task sched tsk_a i) eqn:SCHEDa;
-              [apply eq_leq; symmetry | by ins].
-            apply/eqP; rewrite eqb1.
-            by apply/hasP; exists tsk_a; last by apply/andP.
+            apply leq_sum_nat; move => t /andP [GEt LTt] _.
+            destruct (backlogged job_cost job_jitter sched j t) eqn:BACK;
+              last by rewrite (eq_bigr (fun x => 0)); [by simpl_sum_const | by ins].
+            destruct ([exists cpu, task_scheduled_on job_task sched tsk_a cpu t]) eqn:SCHED;
+              last first.
+            {
+              apply negbT in SCHED; rewrite negb_exists in SCHED; move: SCHED => /forallP ALL.
+              rewrite (eq_bigr (fun x => 0)); first by simpl_sum_const.
+              by intros cpu _; specialize (ALL cpu); apply negbTE in ALL; rewrite ALL.
+            }
+            move: SCHED => /existsP [cpu SCHED].
+            apply leq_trans with (n := 1); last first.
+            {
+              rewrite lt0b; apply/hasP; exists tsk_a; first by done.
+              by rewrite LEa 2!andTb; apply/existsP; exists cpu.
+            }
+            rewrite (bigD1 cpu) /= // SCHED.
+            rewrite (eq_bigr (fun x => 0)); first by simpl_sum_const; rewrite leq_b1.
+            intros cpu' DIFF.
+            apply/eqP; rewrite eqb0; apply/negP.
+            intros SCHED'. 
+            move: DIFF => /negP DIFF; apply DIFF; apply/eqP.
+            unfold task_scheduled_on in *.
+            destruct (sched cpu t) as [j1|] eqn:SCHED1; last by done.
+            destruct (sched cpu' t) as [j2|] eqn:SCHED2; last by done.
+            move: SCHED SCHED' => /eqP JOB /eqP JOB'.
+            subst tsk_a; symmetry in JOB'.
+            assert (PENDING1: pending job_cost job_jitter sched j1 t).
+            {
+              apply scheduled_implies_pending; try by done.
+              by apply/existsP; exists cpu; apply/eqP.
+            }
+            assert (PENDING2: pending job_cost job_jitter sched j2 t).
+            {
+              apply scheduled_implies_pending; try by done.
+              by apply/existsP; exists cpu'; apply/eqP.
+            }
+            assert (BUG: j1 = j2).
+            {
+              apply platform_at_most_one_pending_job_of_each_task with (task_cost0 := task_cost)
+               (job_jitter0 := job_jitter) (task_period0 := task_period) (job_cost0 := job_cost)
+               (task_deadline0 := task_deadline) (tsk0 := tsk) (job_task0 := job_task) (sched0 := sched)
+               (j0 := j) (t0 := t);
+              rewrite ?JOBtsk ?SAMEtsk //; first by apply PARAMS; rewrite -JOBtsk FROMTS.
+              intros j0 tsk0 TSK0 LE.
+              by apply (bertogna_edf_all_previous_jobs_complete_by_their_period t); rewrite ?TSK0.
+            }
+            by subst j2; apply SEQ with (j := j1) (t := t).
           }
-          apply leq_trans with (\sum_(t1 <= t < t1 + R)
-                                     total_interference_B t).
+
+          apply leq_trans with (\sum_(t1 <= t < t1 + R) total_interference_B t).
           {
             rewrite big_distrl /=.
-            rewrite big_nat_cond [\sum_(_ <= _ < _ | true)_]big_nat_cond.
-            apply leq_sum; move => t /andP [LEt _].
+            apply leq_sum_nat; move => t LEt _.
             unfold some_interference_A, total_interference_B. 
             destruct (backlogged job_cost job_jitter sched j t) eqn:BACK;
-              [rewrite andTb mul1n | by done].
+              [rewrite mul1n /= | by rewrite has_pred0 //].
+
             destruct (has (fun tsk_k : sporadic_task => (delta <= x tsk_k) &&
                        task_is_scheduled job_task sched tsk_k t) ts_interf) eqn:HAS';
               last by done.
-            rewrite mul1n; move: HAS => /hasP HAS.
-            destruct HAS as [tsk_k INk LEk].
-
-            have COUNT := bertogna_edf_scheduling_invariant t LEt BACK.
-
+            rewrite mul1n; move: HAS => /hasP [tsk_k INk LEk].
             unfold cardGE.
-            set interfering_tasks_at_t :=
-              [seq tsk_k <- ts_interf | task_is_scheduled job_task
-                                                          sched tsk_k t].
-
-            rewrite -(count_filter (fun i => true)) in COUNT.
-            fold interfering_tasks_at_t in COUNT.
-            rewrite count_predT in COUNT.
             apply leq_trans with (n := num_cpus -
                          count (fun i => (x i >= delta) &&
                             task_is_scheduled job_task sched i t) ts_interf).
@@ -447,48 +589,32 @@ Module ResponseTimeAnalysisEDFJitter.
               rewrite -2!sum1_count big_mkcond /=.
               rewrite [\sum_(_ <- _ | _ <= _)_]big_mkcond /=.
               apply leq_sum; intros i _.
-              destruct (task_is_scheduled job_task sched i t);
+              by destruct (task_is_scheduled job_task sched i t);
                 [by rewrite andbT | by rewrite andbF].
             }
-
-            rewrite leq_subLR -count_predUI.
-            apply leq_trans with (n :=
-                count (predU (fun i : sporadic_task =>
-                                (delta <= x i) &&
-                                task_is_scheduled job_task sched i t)
-                             (fun tsk_k0 : sporadic_task =>
-                                (x tsk_k0 < delta) &&
-                                task_is_scheduled job_task sched tsk_k0 t))
-                      ts_interf); last by apply leq_addr.
-            apply leq_trans with (n := size interfering_tasks_at_t).
-            {
-              rewrite -COUNT.
-              rewrite leq_eqVlt; apply/orP; left; apply/eqP; f_equal.
-              unfold interfering_tasks_at_t.
-              rewrite -filter_predI; apply eq_filter; red; simpl.
-              by intros i; rewrite andbC.
-            }
-            unfold interfering_tasks_at_t.
-            rewrite -count_predT count_filter.
-            rewrite leq_eqVlt; apply/orP; left; apply/eqP.
-            apply eq_count; red; simpl.
-            intros i.
-            destruct (task_is_scheduled job_task sched i t);
-              rewrite 3?andTb ?andFb ?andbF ?andbT /=; try ins.
-            by rewrite leqNgt orNb. 
+            rewrite -count_filter -[count _ ts_interf]count_filter.
+            eapply leq_trans with (n := count (predC (fun tsk => delta <= x tsk)) _);
+              last by apply eq_leq, eq_in_count; red; ins; rewrite ltnNge.
+            rewrite leq_subLR count_predC size_filter.
+            apply leq_trans with (n := count (scheduled_task_other_than_tsk t) ts);
+              first by rewrite bertogna_edf_scheduling_invariant.
+            by rewrite count_filter.
           }
           {
-              unfold x at 2, task_interference.
-              rewrite exchange_big /=; apply leq_sum; intros t _.
-              unfold total_interference_B.
-              destruct (backlogged job_cost job_jitter sched j t); last by ins.
-              rewrite mul1n -sum1_count.
-              rewrite big_seq_cond big_mkcond [\sum_(i <- ts_interf | _ < _) _]big_mkcond.
-              by apply leq_sum; ins; clear -i; desf; des; rewrite ?Heq2.
+            unfold x at 2, total_interference_B.
+            rewrite exchange_big /=; apply leq_sum; intros t _.
+            destruct (backlogged job_cost job_jitter sched j t) eqn:BACK; last by ins.
+            rewrite mul1n -sum1_count.
+            rewrite big_mkcond [\sum_(i <- ts_interf | _ < _) _]big_mkcond /=.
+            apply leq_sum_seq; move => tsk_k IN _.
+            destruct (x tsk_k < delta); [rewrite andTb | by rewrite andFb].
+            destruct (task_is_scheduled job_task sched tsk_k t) eqn:SCHED; last by done.
+            move: SCHED => /existsP [cpu SCHED].
+            by rewrite (bigD1 cpu) /= // SCHED.
           }
         Qed.
 
-        (* 4) Next, we prove that, for any interval delta, if the sum of per-task
+        (* 6) Next, we prove that, for any interval delta, if the sum of per-task
               interference exceeds delta * num_cpus, the same applies for the
               sum of the minimum between the interference and delta. *)
         Lemma bertogna_edf_minimum_exceeds_interference :
@@ -534,10 +660,11 @@ Module ResponseTimeAnalysisEDFJitter.
           apply leq_trans with (n := delta * cardGE delta +
                                      delta * (num_cpus - cardGE delta));
             first by rewrite -mulnDr subnKC //; apply ltnW.
-          by rewrite leq_add2l; apply bertogna_edf_helper_lemma; rewrite -has_count.
+          rewrite leq_add2l; apply bertogna_edf_helper_lemma.
+          by apply/andP; split; first by rewrite -has_count.
         Qed.
 
-        (* 5) Now, we prove that the Bertogna's interference bound
+        (* 7) Now, we prove that the Bertogna's interference bound
               is not enough to cover the sum of the "minimum" term over
               all tasks (artifact of the proof by contradiction). *)
         Lemma bertogna_edf_sum_exceeds_total_interference:
@@ -581,7 +708,7 @@ Module ResponseTimeAnalysisEDFJitter.
           by apply bertogna_edf_too_much_interference.
         Qed.
 
-        (* 6) After concluding that the sum of the minimum exceeds (R - e_i + 1),
+        (* 8) After concluding that the sum of the minimum exceeds (R - e_i + 1),
               we prove that there exists a tuple (tsk_k, R_k) such that
               min (x_k, R - e_i + 1) > min (W_k, edf_bound, R - e_i + 1). *)
         Lemma bertogna_edf_exists_task_that_exceeds_bound :
