model/basic/platform_fp.v
@@ -206,7 +206,7 @@ Module PlatformFP.
           apply count_exists; first by done.
           {
             intros cpu x1 x2 SCHED1 SCHED2.
-            unfold schedules_job_of_task in *.
+            unfold task_scheduled_on in *.
             destruct (sched cpu t); last by done.
             move: SCHED1 SCHED2 => /eqP SCHED1 /eqP SCHED2.
             by rewrite -SCHED1 -SCHED2.
@@ -248,9 +248,8 @@ Module PlatformFP.
             rewrite mem_scheduled_jobs_eq_scheduled in SCHED'.
             apply/andP; split.
             {
-              move: SCHED' => /exists_inP [cpu INcpu /eqP SCHED'].
-              apply/exists_inP; exists cpu; first by done.
-              by unfold schedules_job_of_task; rewrite SCHED' eq_refl.
+              move: SCHED' => /existsP [cpu /eqP SCHED'].
+              by apply/existsP; exists cpu; rewrite /task_scheduled_on SCHED' eq_refl.
             }
             apply/andP; split; first by rewrite -JOBtsk; apply PRIO with (t := t).
             {
