model/jitter/platform.v
@@ -6,7 +6,7 @@ Require Import ssreflect ssrbool ssrfun eqtype ssrnat seq fintype bigop.
 
 Module Platform.
 
-  Import Job SporadicTaskset ScheduleWithJitter ScheduleOfSporadicTask SporadicTaskset SporadicTaskArrival Interference Priority.
+  Import Job SporadicTaskset ScheduleOfSporadicTaskWithJitter SporadicTaskset SporadicTaskArrival Interference Priority.
 
   Section SchedulingInvariants.
     
@@ -281,7 +281,6 @@ Module Platform.
             apply count_exists; first by done.
             {
               intros cpu x1 x2 SCHED1 SCHED2.
-              unfold schedules_job_of_tsk in *.
               destruct (sched cpu t); last by done.
               move: SCHED1 SCHED2 => /eqP SCHED1 /eqP SCHED2.
               by rewrite -SCHED1 -SCHED2.
@@ -309,9 +308,8 @@ Module Platform.
               rewrite mem_scheduled_jobs_eq_scheduled in SCHED'.
               unfold scheduled_task_other_than; apply/andP; split.
               {
-                move: SCHED' => /exists_inP [cpu INcpu /eqP SCHED'].
-                apply/exists_inP; exists cpu; first by done.
-                by unfold schedules_job_of_tsk; rewrite SCHED' eq_refl.
+                move: SCHED' => /existsP [cpu /eqP SCHED'].
+                by apply/existsP; exists cpu; rewrite /task_scheduled_on SCHED' eq_refl.
               }
               {
                 apply/eqP; red; intro SAMEtsk; symmetry in SAMEtsk.
