model/jitter/platform_fp.v
@@ -7,7 +7,7 @@ Require Import ssreflect ssrbool ssrfun eqtype ssrnat seq fintype bigop.
 
 Module PlatformFP.
 
-  Import Job SporadicTaskset ScheduleWithJitter ScheduleOfSporadicTask SporadicTaskset
+  Import Job SporadicTaskset ScheduleOfSporadicTaskWithJitter SporadicTaskset
          SporadicTaskArrival Interference Priority Platform.
 
   Section Lemmas.
@@ -217,7 +217,6 @@ Module PlatformFP.
           apply count_exists; first by done.
           {
             intros cpu x1 x2 SCHED1 SCHED2.
-            unfold schedules_job_of_tsk in *.
             destruct (sched cpu t); last by done.
             move: SCHED1 SCHED2 => /eqP SCHED1 /eqP SCHED2.
             by rewrite -SCHED1 -SCHED2.
@@ -261,9 +260,8 @@ Module PlatformFP.
             rewrite mem_scheduled_jobs_eq_scheduled in SCHED'.
             apply/andP; split.
             {
-              move: SCHED' => /exists_inP [cpu INcpu /eqP SCHED'].
-              apply/exists_inP; exists cpu; first by done.
-              by unfold schedules_job_of_tsk; rewrite SCHED' eq_refl.
+              move: SCHED' => /existsP [cpu /eqP SCHED'].
+              by apply/existsP; exists cpu; rewrite /task_scheduled_on SCHED' eq_refl.
             }
             apply/andP; split; first by rewrite -JOBtsk; apply PRIO with (t := t).
             {
